Readme.md
@@ -10,6 +10,7 @@ Goals:
 - Add pairs, sums, unit, void, nats, primrec? sructured types?
 - Make printing part of the code
 - Make initialization part of the code
+- Let-polymorphism
 
 Refactorings: 
 
